Refinery/Term/Extrinsic/Refinement/Arrow/Premonoidal/Binoidal.lean
@@ -1,0 +1,217 @@
+import Refinery.Term.Extrinsic.Refinement.Arrow.Premonoidal.Structure
+
+open HasQuant HasPQuant HasCommRel
+
+namespace Refinery
+
+namespace Term
+
+variable {φ : Type u} {α : Type v} {ε : Type w} [S : Signature φ α ε] {R : DRWS φ α} [R.UWkCongr]
+
+theorem DRWS.Obj.whiskerLeft_id (A : R.Obj) : A.id.whiskerLeft B = id (B.tensor A)
+  := by simp [Arrow.whiskerLeft, Eqv.letT₂, Eqv.letArrow_id]; exact Eqv.let₂_eta _
+
+theorem DRWS.Obj.id_whiskerRight (A : R.Obj) : A.id.whiskerRight B = id (A.tensor B)
+  := by
+  simp [Arrow.whiskerRight, Eqv.letArrow_id]
+  convert Eqv.let₂_eta _ using 1
+  apply Eqv.sound; apply Wf.eqv.of_tm; rfl
+
+theorem Eqv.letArrow_whiskerLeft
+  (a : Eqv R Γ (A.tensor B)) (f : DRWS.Arrow R B C)
+  : a.letArrow (f.whiskerLeft A) = .letT₂ a (.pair
+    ((Ctx?.erase_right _).cons (.right _))
+    .bv1 (.letArrow .bv0 f)
+  ) := by
+  apply Eq.symm
+  convert a.bind_let₂ _ _
+  induction a, f using quotInd₂
+  apply sound; apply Wf.eqv.of_tm;
+  simp only [
+    Wf.let₁, Wf.wk, Wf.let₂, Wf.pair, Wf.bv1, Wf.bv0, Wf.wk2, Ctx?.extend1, Ctx?.Wk.ix,
+    Ctx?.Wk.drop_ix, Ctx?.length
+  ]
+  simp [Ctx?.nil, Ctx?.cons, Ctx?.erase, ren_ren, <-Nat.liftWk_comp]
+  rfl
+
+theorem Eqv.letArrow_whiskerRight
+  (a : Eqv R Γ (A.tensor B)) (f : DRWS.Arrow R A C)
+  : a.letArrow (f.whiskerRight B) = .letT₂ a (.pair
+    (((Ctx?.erase_left _).cons (.left _)).cons (.right _))
+     (.letArrow .bv1 f) .bv0
+  ) := by
+  apply Eq.symm
+  convert a.bind_let₂ _ _
+  induction a, f using quotInd₂
+  apply sound; apply Wf.eqv.of_tm;
+  simp only [
+    Wf.let₁, Wf.wk, Wf.let₂, Wf.pair, Wf.bv1, Wf.bv0, Wf.wk2, Ctx?.extend1, Ctx?.Wk.ix,
+    Ctx?.Wk.drop_ix, Ctx?.length
+  ]
+  simp [Ctx?.nil, Ctx?.cons, Ctx?.erase, ren_ren, <-Nat.liftWk_comp]
+  rfl
+
+theorem DRWS.Arrow.whiskerLeft_comp_whiskerLeft {A : R.Obj}
+  (f : Arrow R B C) (g : Arrow R C D)
+  : (f.whiskerLeft A).comp (g.whiskerLeft A) = (f.comp g).whiskerLeft A
+  := by
+  rw [
+    comp, Eqv.letArrow_whiskerLeft, whiskerLeft, Eqv.toEqv_toArr, Eqv.letT₂, Eqv.letT₂,
+    Eqv.let₂_let₂, whiskerLeft]
+  congr 2
+  conv => rhs; rw [Eqv.bind_pair]
+  rw [Eqv.let₂_beta]
+  congr 1
+  simp only [
+    Eqv.wk0_letArrow, Eqv.wk0_bv0, Eqv.let_letArrow, comp, Eqv.toArr, extend1, Eqv.wk_letArrow,
+    toEqv
+  ]
+  congr 2
+  rw [bv0_letArrow']
+  conv => lhs;
+  simp only [Eqv.wk2_pair, Eqv.wk1_pair, Eqv.wk1_bv1, Eqv.wk2_bv1, Eqv.wk1_bv0]
+  apply Eq.symm
+  generalize (Ctx?.SSplit.cons (α := α) _ _) = hΓ₁
+  generalize (Ctx?.SSplit.cons (α := α) _ _) = hΓ₂
+  generalize (Ctx?.SSplit.cons (α := α) _ _) = hΓ₃
+  generalize hρ : (Ctx?.extend1 (hΓ := _) (α := α) _ _) = ρ
+  induction f, g using Eqv.quotInd₂ with
+  | h f g =>
+  apply Eqv.sound
+  apply ((g.wk ρ).pre_beta_pureLout hΓ₁
+    (Wf.pair (.cons (.cons (.cons (Ctx?.erase_right _) (.left _)) (.left _)) (.right _))
+      .bv3 .bv0) (hb := _)).coh
+  rfl
+  simp [
+    Wf.pair, Wf.wk1, Wf.subst, Wf.wk, Wf.bv3, Wf.bv2, Wf.wk2, SubstDS.refl_get, Wf.bv0,
+    Ctx?.extend1, ren_ren, <-Nat.liftWk_comp, <-hρ
+  ]
+  rfl
+  reduce
+  infer_instance
+
+theorem DRWS.Arrow.whiskerLeft_comp {A : R.Obj} (f : Arrow R B C) (g : Arrow R C D)
+  : (f.comp g).whiskerLeft A = (f.whiskerLeft A).comp (g.whiskerLeft A)
+  := (f.whiskerLeft_comp_whiskerLeft g).symm
+
+theorem DRWS.Arrow.whiskerRight_comp_whiskerRight {A : R.Obj}
+  (f : Arrow R B C) (g : Arrow R C D)
+  : (f.whiskerRight A).comp (g.whiskerRight A) = (f.comp g).whiskerRight A := by
+  rw [
+    comp, Eqv.letArrow_whiskerRight, whiskerRight, Eqv.toEqv_toArr, Eqv.letT₂, Eqv.letT₂,
+    Eqv.let₂_let₂, whiskerRight, Eqv.letArrow_comp
+  ]
+  congr 2
+  conv => rhs; rw [Eqv.bind_pair_left]
+  rw [Eqv.let₂_beta]
+  conv => rhs; rw [Eqv.let_letArrow]
+  congr 1
+  rw [Eqv.bind_pair_left, Eqv.let_letArrow, Eqv.wk0_bv0]
+  apply Eq.trans _ (Eqv.swap0_swap0 _)
+  rw [Eqv.swap0, Eqv.swap0]
+  induction g using Eqv.quotInd
+  apply Eqv.of_tm
+  simp [Wf.let₁, Wf.wk2, Wf.wk, Wf.wk1, Wf.pair, Wf.bv0, ren_ren, Wf.wk0, Ctx?.extend1, Wf.bv1]
+  congr 1
+  ext x; cases x <;> rfl
+
+theorem DRWS.Arrow.comp_whiskerRight {A : R.Obj} (f : Arrow R B C) (g : Arrow R C D)
+  : (f.comp g).whiskerRight A = (f.whiskerRight A).comp (g.whiskerRight A)
+  := (f.whiskerRight_comp_whiskerRight g).symm
+
+theorem Eqv.letArrow_tensorHom {A B A' B' : Ty α}
+  (a : Eqv R Γ (A.tensor A')) (f : R.Arrow A B) (g : R.Arrow A' B')
+  : a.letArrow (f.tensorHom g) = .letT₂ a (.pair
+    (((Ctx?.erase_left _).cons (.left _)).cons (.right _))
+     (.letArrow .bv1 f) (.letArrow .bv0 g)
+  ) := by
+  apply Eq.symm
+  convert a.bind_let₂ _ _
+  induction a, f, g using quotInd₃
+  apply sound; apply Wf.eqv.of_tm;
+  simp only [
+    Wf.let₁, Wf.wk, Wf.let₂, Wf.pair, Wf.bv1, Wf.bv0, Wf.wk2, Ctx?.extend1, Ctx?.Wk.ix,
+    Ctx?.Wk.drop_ix, Ctx?.length
+  ]
+  simp [Ctx?.nil, Ctx?.cons, Ctx?.erase, ren_ren, <-Nat.liftWk_comp]
+  constructor <;> rfl
+
+def DRWS.Arrow.ltimes {A B A' B' : Ty α} (f : Arrow R A A') (g : Arrow R B B')
+  : Arrow R (A.tensor B) (A'.tensor B') := (f.whiskerRight _).comp (g.whiskerLeft _)
+
+theorem DRWS.Arrow.tensorHom_eq_ltimes {A B A' B' : Ty α} (f : Arrow R A A') (g : Arrow R B B')
+  : f.tensorHom g = f.ltimes g := by
+  rw [
+    ltimes, comp, Eqv.letArrow_whiskerLeft, whiskerRight, Eqv.toEqv_toArr, Eqv.letT₂_letT₂,
+    Eqv.letT₂_beta, tensorHom
+  ]
+  congr 2
+  rw [Eqv.bind_pair_left]
+  congr 1
+  apply Eq.symm
+  induction g using Eqv.quotInd with
+  | h hg =>
+  apply Eqv.sound
+  apply Wf.eqv.coh_out
+  apply Wf.pre_beta_pureIIn
+  simp
+  simp [
+    Wf.subst, Wf.pair, Wf.bv0, Wf.wk0, Wf.let₁, Wf.wk2, Wf.wk, Wf.bv1, SubstDS.refl_get, ren_ren,
+  ]
+  rw [<-subst_renIn, <-subst_ofRen]
+  apply Subst.subst_eqOn_fvi
+  intro x hx
+  cases x
+  rfl
+  have hg := hg.deriv.fvi_le_length
+  simp at hg
+  omega
+
+def DRWS.Arrow.rtimes {A B A' B' : Ty α} (f : Arrow R A A') (g : Arrow R B B')
+  : Arrow R (A.tensor B) (A'.tensor B') := (g.whiskerLeft _).comp (f.whiskerRight _)
+
+def DRWS.Arrow.tensorHomLeft {A B C A' B' C'}
+  (f : Arrow R A A') (g : Arrow R B B') (h : Arrow R C C')
+  : Arrow R ((A.tensor B).tensor C) ((A'.tensor B').tensor C')
+  := Eqv.toArr (.letT₂ .bv0 (.let₂ (Ctx?.erase_left _).right.left .bv1 (
+    .pair (Ctx?.erase_left _).left.left
+    (.pair (Ctx?.erase_right _).right (.letArrow .bv1 f) (.letArrow .bv0 g)) (.letArrow .bv2 h)
+  )))
+
+def DRWS.Arrow.tensorHomRight  {A B C A' B' C'}
+  (f : Arrow R A A') (g : Arrow R B B') (h : Arrow R C C')
+  : Arrow R (A.tensor (B.tensor C)) (A'.tensor (B'.tensor C'))
+  := Eqv.toArr (.letT₂ .bv0 (.let₂ (Ctx?.erase_right _).right .bv0 (
+    .pair (Ctx?.erase_right _).right.right (.letArrow .bv3 f)
+      (.pair (Ctx?.erase_right _).right (.letArrow .bv1 g) (.letArrow .bv0 h))
+  )))
+
+def DRWS.Arrow.tensorHomSwap0 (f : Arrow R A A') (g : Arrow R B B')
+  : Arrow R (A.tensor B) (A'.tensor B')
+  := Eqv.toArr (.letT₂ (.reswap .bv0) (Eqv.pair
+    (((Ctx?.erase_left _).cons (.left _)).cons (.right _))
+     (.letArrow .bv1 f) (.letArrow .bv0 g)
+  ).swap0)
+
+theorem DRWS.Arrow.tensorHom_eq_swap0 (f : Arrow R A A') (g : Arrow R B B')
+  : f.tensorHom g = f.tensorHomSwap0 g
+  := by
+  rw [tensorHom, tensorHomSwap0, Eqv.letT₂, Eqv.letT₂, Eqv.let₂_reswap, Eqv.swap0_swap0]
+  rfl
+
+def DRWS.Arrow.tensorHomReswap (f : Arrow R A A') (g : Arrow R B B')
+  : Arrow R (A.tensor B) (A'.tensor B')
+  := Eqv.toArr (.letT₂ (.reswap .bv0) (.pair
+    (((Ctx?.erase_left _).cons (.right _)).cons (.left _))
+     (.letArrow .bv0 f) (.letArrow .bv1 g)
+  ))
+
+-- theorem DRWS.Arrow.tensorHom_eq_reswap (f : Arrow R A B) (g : Arrow R A' B')
+--   : f.tensorHom g = f.tensorHomReswap g
+--   := sorry
+
+def DRWS.Arrow.rtensorHom (f : Arrow R A A') (g : Arrow R B B')
+  : Arrow R (A.tensor B) (A'.tensor B') := Eqv.toArr (.letT₂ .bv0 (.antipair
+    (((Ctx?.erase_left _).cons (.left _)).cons (.right _))
+     (.letArrow .bv1 f) (.letArrow .bv0 g)
+  ))
