Refinery/Term/Extrinsic/Refinement/Arrow/Premonoidal/Structure.lean
@@ -1,0 +1,568 @@
+import Refinery.Term.Extrinsic.Refinement.Arrow.Category
+import Refinery.Term.Extrinsic.Wf.DerivedRewrite
+import Refinery.Term.Extrinsic.Wf.Swap
+import Discretion.Premonoidal.Category
+
+open HasQuant HasPQuant HasCommRel
+
+namespace Refinery
+
+namespace Term
+
+variable {φ : Type u} {α : Type v} {ε : Type w} [S : Signature φ α ε] {R : DRWS φ α} [R.UWkCongr]
+
+def DRWS.Arrow.whiskerLeft (A : R.Obj) (f : Arrow R B C) : Arrow R (A.tensor B) (A.tensor C)
+  := Eqv.toArr (.letT₂ .bv0 (.pair
+    ((Ctx?.erase_right _).cons (.right _))
+    .bv1 (.letArrow .bv0 f)
+  ))
+
+def DRWS.Arrow.whiskerRight (f : Arrow R A B) (C : R.Obj) : Arrow R (A.tensor C) (B.tensor C)
+  := Eqv.toArr (.letT₂ .bv0 (.pair
+    (((Ctx?.erase_left _).cons (.left _)).cons (.right _))
+     (.letArrow .bv1 f) .bv0
+  ))
+
+def DRWS.Arrow.tensorHom (f : Arrow R A B) (g : Arrow R A' B')
+  : Arrow R (A.tensor A') (B.tensor B')
+  := Eqv.toArr (.letT₂ .bv0 (.pair
+    (((Ctx?.erase_left _).cons (.left _)).cons (.right _))
+     (.letArrow .bv1 f) (.letArrow .bv0 g)
+  ))
+
+def Eqv.releft {Γ : Ctx? α} {A : Ty α}
+  (a : Eqv R Γ (.tensor .unit A)) : Eqv R Γ A
+  := .letT₂ a .bv0
+
+def Eqv.releft_inv {Γ : Ctx? α} {A : Ty α}
+  (a : Eqv R Γ A) : Eqv R Γ (.tensor .unit A)
+  := .pair (Ctx?.erase_left _) (.unit _) a
+
+theorem Eqv.releft_inv_releft {Γ : Ctx? α} {A : Ty α}
+  (a : Eqv R Γ A) : a.releft_inv.releft = a := by
+  rw [releft_inv, releft, letT₂, let₂_beta]
+  conv => rhs; rw [<-let₁_eta a, let₁_unit_anti (let₁ _ _ _)]
+  induction a using quotInd
+  apply Eqv.sound; apply Wf.eqv.of_tm
+  rfl
+
+theorem Eqv.releft_releft_inv {Γ : Ctx? α} {A : Ty α}
+  (a : Eqv R Γ (.tensor .unit A)) : a.releft.releft_inv = a := by
+  rw [releft, releft_inv]
+  conv => rhs; rw [<-letT₂_eta a]; rhs; lhs; rw [bv1.unit_pure_del (hΓ := by
+    rw [Ctx?.cons_del_iff]
+    constructor
+    rw [Ctx?.cons_del_iff]
+    constructor
+    infer_instance
+    apply Var?.del.instTopQuant
+    infer_instance
+  )]
+  rw [bind_pair_right _ ⊥ ⊤, letT₂, let_let₂, letT₂]
+  conv => rhs; rhs; rw [<-let₁_bv0 (.pair _ _ _)]
+  induction a using quotInd
+  apply Eqv.sound; apply Wf.eqv.of_tm
+  rfl
+  apply HasCommRel.commutes_bot_left
+
+def DRWS.Obj.leftUnitor (A : R.Obj) : Arrow R (.tensor .unit A) A
+  := Eqv.toArr (Eqv.bv0.releft)
+
+def DRWS.Obj.leftUnitor_inv (A : R.Obj) : Arrow R A (.tensor .unit A)
+  := Eqv.toArr (Eqv.bv0.releft_inv)
+
+theorem Eqv.letArrow_leftUnitor {Γ : Ctx? α} {A : Ty α}
+  (a : Eqv R Γ (.tensor .unit A)) : a.letArrow (DRWS.Obj.leftUnitor A) = a.releft
+  := by
+  rw [releft, letT₂, bind_let₂]
+  induction a using quotInd
+  exact Eqv.of_tm rfl
+
+theorem Eqv.letArrow_leftUnitor_inv {Γ : Ctx? α} {A : Ty α}
+  (a : Eqv R Γ A) : a.letArrow (DRWS.Obj.leftUnitor_inv A) = a.releft_inv
+  := by
+  rw [releft_inv, bind_pair_right _ ⊥ ⊤]
+  induction a using quotInd
+  exact Eqv.of_tm rfl
+  apply HasCommRel.commutes_bot_left
+
+theorem DRWS.Obj.leftUnitor_leftUnitor_inv {A : R.Obj}
+  : A.leftUnitor.comp A.leftUnitor_inv = id (.tensor .unit A) := by
+  simp [DRWS.Arrow.comp, Eqv.letArrow_leftUnitor_inv, leftUnitor, Eqv.releft_releft_inv]
+  rfl
+
+theorem DRWS.Obj.leftUnitor_inv_leftUnitor {A : R.Obj}
+  : A.leftUnitor_inv.comp A.leftUnitor = id A := by
+  simp [DRWS.Arrow.comp, Eqv.letArrow_leftUnitor, leftUnitor_inv, Eqv.releft_inv_releft]
+  rfl
+
+def Eqv.reright {Γ : Ctx? α} {A : Ty α}
+  (a : Eqv R Γ (A.tensor .unit)) : Eqv R Γ A
+  := .letT₂ a .bv1
+
+def Eqv.reright_inv {Γ : Ctx? α} {A : Ty α}
+  (a : Eqv R Γ A) : Eqv R Γ (A.tensor .unit)
+  := .pair (Ctx?.erase_right _) a (.unit _)
+
+theorem Eqv.reright_reright_inv {Γ : Ctx? α} {A : Ty α}
+  (a : Eqv R Γ A) : a.reright_inv.reright = a := by
+  rw [reright_inv, reright, letT₂, let₂_beta]
+  conv => rhs; rw [<-let₁_eta a, let₁_unit_anti .bv0]
+  induction a using quotInd
+  exact Eqv.of_tm rfl
+
+theorem Eqv.reright_inv_reright {Γ : Ctx? α} {A : Ty α}
+  (a : Eqv R Γ (A.tensor .unit)) : a.reright.reright_inv = a := by
+  rw [reright, reright_inv, letT₂, let₂_pair_right]
+  conv => rhs; rw [<-a.let₂_eta]
+  rw [bv0.unit_pure_del]
+  induction a using quotInd
+  exact Eqv.of_tm rfl
+
+def DRWS.Obj.rightUnitor (A : R.Obj) : Arrow R (A.tensor .unit) A
+  := Eqv.toArr (Eqv.bv0.reright)
+
+def DRWS.Obj.rightUnitor_inv (A : R.Obj) : Arrow R A (A.tensor .unit)
+  := Eqv.toArr (Eqv.bv0.reright_inv)
+
+theorem Eqv.letArrow_rightUnitor {Γ : Ctx? α} {A : Ty α}
+  (a : Eqv R Γ (A.tensor .unit)) : a.letArrow (DRWS.Obj.rightUnitor A) = a.reright
+  := by
+  rw [reright, letT₂, bind_let₂]
+  induction a using quotInd
+  exact Eqv.of_tm rfl
+
+theorem Eqv.letArrow_rightUnitor_inv {Γ : Ctx? α} {A : Ty α}
+  (a : Eqv R Γ A) : a.letArrow (DRWS.Obj.rightUnitor_inv A) = a.reright_inv
+  := by
+  rw [reright_inv, bind_pair_left]
+  induction a using quotInd
+  exact Eqv.of_tm rfl
+
+theorem DRWS.Obj.rightUnitor_rightUnitor_inv {A : R.Obj}
+  : A.rightUnitor.comp A.rightUnitor_inv = id (A.tensor .unit) := by
+  simp [DRWS.Arrow.comp, Eqv.letArrow_rightUnitor_inv, rightUnitor, Eqv.reright_inv_reright]
+  rfl
+
+theorem DRWS.Obj.rightUnitor_inv_rightUnitor {A : R.Obj}
+  : A.rightUnitor_inv.comp A.rightUnitor = id A := by
+  simp [DRWS.Arrow.comp, Eqv.letArrow_rightUnitor, rightUnitor_inv, Eqv.reright_reright_inv]
+  rfl
+
+def Eqv.reassoc {Γ : Ctx? α} {A B C : Ty α}
+  (a : Eqv R Γ ((A.tensor B).tensor C))
+  : Eqv R Γ (A.tensor (B.tensor C))
+  := .letT₂ a (
+    .let₂ ((Ctx?.erase_left _).cons (.left _)) .bv1 (.pair
+      ((((Ctx?.erase_left _).cons (.right _)).cons (.left _)).cons (.right _))
+      .bv1
+      (.pair
+        ((((Ctx?.erase_left _).cons (.right _)).cons (.left _)).cons (.left _))
+        .bv0
+        .bv2
+      ))
+  )
+
+def Eqv.reassoc_inv {Γ : Ctx? α} {A B C : Ty α}
+  (a : Eqv R Γ (A.tensor (B.tensor C)))
+  : Eqv R Γ ((A.tensor B).tensor C)
+  := .let₂ (Ctx?.erase_left _) a (
+    .let₂ ((Ctx?.erase_right _).cons (.right _)) .bv0 (.pair
+      ((Ctx?.erase_right _).cons (.right _))
+      (.pair
+        ((((Ctx?.erase_right _).cons (.right _)).cons (.right _)).cons (.left _))
+        .bv3 .bv1)
+      .bv0
+    ))
+
+def Eqv.eta_assoc {Γ : Ctx? α} {A B C : Ty α}
+  (a : Eqv R Γ ((A.tensor B).tensor C))
+  : Eqv R Γ ((A.tensor B).tensor C)
+  := .letT₂ a (
+    .let₂ (Ctx?.erase_left _).left .bv1 (.pair
+      (Ctx?.erase_right _).right.left.left
+      (.pair (Ctx?.erase_right _).right .bv1 .bv0)
+      .bv2
+  ))
+
+theorem Eqv.eta_assoc_eq_id {Γ : Ctx? α} {A B C : Ty α}
+  (a : Eqv R Γ ((A.tensor B).tensor C))
+  : a.eta_assoc = a := by
+  rw [Eqv.eta_assoc, letT₂]
+  conv => rhs; rw [<-let₂_eta a]
+  congr 1
+  conv => rhs; lhs; rw [<-let₂_eta .bv1]
+  rw [let₂_pair_right]
+  exact Eqv.of_tm rfl
+
+def Eqv.eta_assoc_inv {Γ : Ctx? α} {A B C : Ty α}
+  (a : Eqv R Γ (A.tensor (B.tensor C)))
+  : Eqv R Γ (A.tensor (B.tensor C))
+  := letT₂ a (
+    .let₂ ((Ctx?.erase_right _).cons (.right _)) .bv0 (.pair
+      (Ctx?.erase_right _).right.right
+      .bv3
+      (.pair (Ctx?.erase_right _).right .bv1 .bv0)
+    ))
+
+theorem Eqv.eta_assoc_inv_eq_id {Γ : Ctx? α} {A B C : Ty α}
+  (a : Eqv R Γ (A.tensor (B.tensor C)))
+  : a.eta_assoc_inv = a := by
+  rw [Eqv.eta_assoc_inv, letT₂]
+  conv => rhs; rw [<-let₂_eta a]
+  congr 1
+  conv =>
+    lhs
+    rw [bind_pair_right _ ⊥ ⊤ (ha := inferInstance) (hb := inferInstance)
+      (he := HasCommRel.commutes_bot_left)]
+  conv =>
+    rhs
+    rw [
+      bind_pair_right _ ⊥ ⊤ (ha := inferInstance) (hb := inferInstance)
+        (he := HasCommRel.commutes_bot_left),
+      <-let₂_eta .bv0, let_let₂
+    ]
+  exact Eqv.of_tm rfl
+
+def DRWS.Obj.assoc (A B C : R.Obj) : Arrow R ((A.tensor B).tensor C) (A.tensor (B.tensor C))
+  := Eqv.toArr (.reassoc .bv0)
+
+def DRWS.Obj.assoc_inv (A B C : R.Obj) : Arrow R (A.tensor (B.tensor C)) ((A.tensor B).tensor C)
+  := Eqv.toArr (.reassoc_inv .bv0)
+
+theorem Eqv.letArrow_assoc {Γ : Ctx? α} {A B C : Ty α}
+  (a : Eqv R Γ ((A.tensor B).tensor C))
+  : a.letArrow (DRWS.Obj.assoc A B C) = a.reassoc
+  := by
+  rw [reassoc, letT₂, bind_let₂]
+  induction a using quotInd
+  apply Eqv.sound; apply Wf.eqv.of_tm
+  simp only [
+    Wf.let₁, Var?.erase_erase, Wf.bv1, Wf.pair, Wf.wk, let₁.injEq, true_and, Wf.let₂, Wf.bv0,
+    Wf.wk2, Wf.bv2]
+  simp [ren_ren, Ctx?.extend1]
+
+theorem Eqv.letArrow_assoc_inv {Γ : Ctx? α} {A B C : Ty α}
+  (a : Eqv R Γ (A.tensor (B.tensor C)))
+  : a.letArrow (DRWS.Obj.assoc_inv A B C) = a.reassoc_inv
+  := by
+  rw [reassoc_inv, bind_let₂]
+  induction a using quotInd
+  apply Eqv.sound; apply Wf.eqv.of_tm
+  simp only [
+    Wf.let₁, Var?.erase_erase, Wf.bv1, Wf.pair, Wf.wk, let₁.injEq, true_and, Wf.let₂, Wf.bv0,
+    Wf.wk2, Wf.bv2, Wf.bv3]
+  simp [ren_ren, Ctx?.extend1]
+
+theorem Eqv.let₂_reassoc {Γ Γl Γr : Ctx? α} {X Y A B C : Ty α}
+  (hΓ : Γ.SSplit Γl Γr)
+  (a : Eqv R Γr (X.tensor Y)) (b : Eqv R ((Γl.cons ⟨X, ⊤⟩).cons ⟨Y, ⊤⟩) ((A.tensor B).tensor C))
+  : (a.let₂ hΓ b).reassoc = a.let₂ hΓ b.reassoc
+  := by
+  rw [reassoc, letT₂, let₂_let₂]
+  induction a, b using quotInd₂
+  apply Eqv.sound; apply Wf.eqv.of_tm
+  rfl
+
+theorem Eqv.let₂_reassoc_inv {Γ Γl Γr : Ctx? α} {X Y A B C : Ty α}
+  (hΓ : Γ.SSplit Γl Γr)
+  (a : Eqv R Γr (X.tensor Y)) (b : Eqv R ((Γl.cons ⟨X, ⊤⟩).cons ⟨Y, ⊤⟩) (A.tensor (B.tensor C)))
+  : (a.let₂ hΓ b).reassoc_inv = a.let₂ hΓ b.reassoc_inv
+  := by
+  rw [reassoc_inv, let₂_let₂]
+  induction a, b using quotInd₂
+  apply Eqv.sound; apply Wf.eqv.of_tm
+  rfl
+
+set_option maxHeartbeats 1000000000 in
+theorem Eqv.reassoc_beta {Γ Γc Γl Γm Γr : Ctx? α} {A B C : Ty α}
+  (hΓ : Γ.SSplit Γc Γr) (hΓc : Γc.SSplit Γl Γm)
+  (a : Eqv R Γl A) (b : Eqv R Γm B) (c : Eqv R Γr C)
+  : ((a.pair hΓc b).pair hΓ c).reassoc = a.pair (hΓ.s12_3_1_23 hΓc) (b.pair (hΓ.s12_3_23 hΓc) c)
+  := calc
+  _ = .let₁ (hΓ.s12_3_1_23 hΓc).comm a
+      (.let₁ ((hΓ.s12_3_23 hΓc).comm.cons (.left _)) (b.wk0 _)
+        (.let₁ ((((Ctx?.erase_left _).comm.cons (.right _))).cons (.right _))
+          (.pair
+            ((((Ctx?.erase_left _).comm.cons (.left _))).cons (.right _))
+            .bv1 .bv0
+          )
+          (.let₁
+            (((Ctx?.erase_right _).comm).cons (.left _)) (((c.wk0 _).wk0 _).wk0 _)
+            (.let₂
+              ((((Ctx?.erase_left _).comm).cons (.right _)).cons (.left _))
+              .bv1
+              (.pair
+                ((((Ctx?.erase_right _).cons (.right _)).cons (.left _)).cons (.right _)) .bv1
+                (.pair
+                  ((((Ctx?.erase_right _).cons (.right _)).cons (.right _)).cons (.left _))
+                  .bv0
+                  .bv2
+                )
+              )
+            )))
+       ) := by
+      rw [reassoc, letT₂, let₂_beta, bind_pair, let_let₁, let_let₁]
+      induction a, b, c using quotInd₃
+      apply Eqv.sound; apply Wf.eqv.of_tm
+      simp [Wf.let₁, Wf.let₂, Wf.pair, Wf.bv1, Wf.wk1, Wf.bv0, Wf.wk0, ren_ren, <-Nat.liftWk_comp]
+      constructor <;> rfl
+  _ = .let₁ (hΓ.s12_3_1_23 hΓc).comm a
+      (.let₁ ((hΓ.s12_3_23 hΓc).comm.cons (.left _)) (b.wk0 _)
+          (.let₁
+            ((((Ctx?.erase_right Γr).comm).cons (.left _)).cons (.left _)) (((c.wk0 _).wk0 _))
+            (.let₂
+              (((((Ctx?.erase_left _).comm).cons
+                (.right ⟨A, ⊤⟩)).cons (.right ⟨B, ⊤⟩)).cons (.left ⟨C, ⊤⟩))
+                (.pair
+                  (((((Ctx?.erase_left _).comm.cons (.left _))).cons (.right _)).cons (.right _))
+                  .bv2 .bv1
+                )
+              (.pair
+                (((((Ctx?.erase_right _).cons
+                  (.right _)).cons (.right ⟨C, ⊤⟩)).cons (.left ⟨A, ⊤⟩)).cons (.right ⟨B, ⊤⟩)) .bv1
+                (.pair
+                  (((((Ctx?.erase_right _).cons
+                    (.right _)).cons (.right ⟨C, ⊤⟩)).cons (.left ⟨A, 0⟩)).cons (.left ⟨B, ⊤⟩))
+                  .bv0
+                  .bv2
+                )
+              )
+            ))
+       ) := by
+        congr 2
+        induction c using quotInd with
+        | h c =>
+        apply sound
+        apply Wf.eqv.coh
+        apply Wf.pre_beta_pureIn
+          ((((Ctx?.erase_left _).comm.cons (.right _))).cons (.right _))
+          (.pair
+            ((((Ctx?.erase_left _).comm.cons (.left _))).cons (.right _))
+            .bv1 .bv0
+          )
+          ⊤
+          (by simp)
+          (.let₁
+            (((Ctx?.erase_right _).comm).cons (.left _)) (((c.wk0 _).wk0 _).wk0 _)
+            (.let₂
+              ((((Ctx?.erase_left _).comm).cons (.right _)).cons (.left _))
+              .bv1
+              (.pair
+                ((((Ctx?.erase_right _).cons (.right _)).cons (.left _)).cons (.right _)) .bv1
+                (.pair
+                  ((((Ctx?.erase_right _).cons (.right _)).cons (.right _)).cons (.left _))
+                  .bv0
+                  .bv2
+                )
+              )
+            ))
+        rfl
+        simp only [
+          Wf.subst, Wf.pair, Wf.bv1, Wf.let₁, Wf.wk0, Wf.let₂, Term.subst, Wf.bv0, Wf.bv2
+        ]
+        simp only [EQuant.coe_top, Subst.get_lift_succ, SubstDS.subst0_get_zero, ren.eq_6, ren,
+          Nat.succ_eq_add_one, Nat.reduceAdd, zero_add, Subst.get_lift_zero, ren.eq_1, let₁.injEq,
+          and_self, and_true]
+        simp only [<-subst_renIn, ren_ren]
+        rw [<-subst_ofRen]
+        apply Subst.subst_eqOn_fvi
+        intro x hx
+        simp [SubstDS.refl_get, lt_of_lt_of_le hx c.deriv.fvi_le_length]
+  _ = let₁ (hΓ.s12_3_1_23 hΓc).comm a
+    (let₁ ((hΓ.s12_3_23 hΓc).comm.cons (Var?.SSplit.left { ty := A, q := ⊤ })) (wk0 _ b)
+      (let₁
+        ((Γr.erase_right.comm.cons
+        (Var?.SSplit.left { ty := A, q := ⊤ })).cons (Var?.SSplit.left { ty := B, q := ⊤ }))
+        (wk0 _ (wk0 _ c))
+        (let₁
+          ((((Γr.erase.erase_left.comm.cons (Var?.SSplit.right { ty := A, q := ⊤ })).cons
+                    (Var?.SSplit.right { ty := B, q := ⊤ })).cons
+                (Var?.SSplit.left { ty := C, q := ⊤ })).s1_23_13_2
+            (((Γr.erase.erase.erase_left.comm.cons (Var?.SSplit.left { ty := A, q := ⊤ })).cons
+                  (Var?.SSplit.right { ty := B, q := ⊤ })).cons
+              (Var?.SSplit.right _)))
+          bv2
+          (let₁
+            (((((Γr.erase.erase_left.comm.cons (Var?.SSplit.right { ty := A, q := ⊤ })).cons
+                          (Var?.SSplit.right { ty := B, q := ⊤ })).cons
+                      (Var?.SSplit.left { ty := C, q := ⊤ })).s1_23_13
+                  (((Γr.erase.erase.erase_left.comm.cons (Var?.SSplit.left { ty := A, q := ⊤ })).cons
+                        (Var?.SSplit.right { ty := B, q := ⊤ })).cons
+                    (Var?.SSplit.right _))).cons
+              (Var?.SSplit.left { ty := A, q := ⊤ }))
+            bv2
+            (pair
+              (((((Γr.erase.cons _).erase_right.cons
+                            (Var?.SSplit.right _)).cons
+                        (Var?.SSplit.right { ty := C, q := ⊤ })).cons
+                    (Var?.SSplit.left { ty := A, q := ⊤ })).cons
+                (Var?.SSplit.right { ty := B, q := ⊤ }))
+              bv1
+              (pair
+                (((((Γr.erase.cons _).erase.erase_right.cons
+                              (Var?.SSplit.right _)).cons
+                          (Var?.SSplit.right { ty := C, q := ⊤ })).cons
+                      (Var?.SSplit.left { ty := A, q := 0 })).cons
+                  (Var?.SSplit.left { ty := B, q := ⊤ }))
+                bv0 bv2)))))) := by rw [let₂_beta]; rfl
+    _ = let₁ (hΓ.s12_3_1_23 hΓc).comm a
+    (let₁ ((hΓ.s12_3_23 hΓc).comm.cons (Var?.SSplit.left { ty := A, q := ⊤ })) (wk0 _ b)
+      (let₁
+        ((Γr.erase_right.comm.cons
+        (Var?.SSplit.left { ty := A, q := ⊤ })).cons (Var?.SSplit.left { ty := B, q := ⊤ }))
+        (wk0 _ (wk0 _ c))
+        (let₁
+          ((((Γr.erase.erase_left.comm.cons (Var?.SSplit.right { ty := A, q := ⊤ })).cons
+                    (Var?.SSplit.right { ty := B, q := ⊤ })).cons
+                (Var?.SSplit.left { ty := C, q := ⊤ })).s1_23_13_2
+            (((Γr.erase.erase.erase_left.comm.cons (Var?.SSplit.left { ty := A, q := ⊤ })).cons
+                  (Var?.SSplit.right { ty := B, q := ⊤ })).cons
+              (Var?.SSplit.right _)))
+          bv2
+          (
+            .pair ((Ctx?.erase_left _).cons (.left _)) .bv0
+              (.pair ((((Ctx?.erase_left _).cons (.left _)).cons (.right _)).cons (.right _))
+                .bv2
+                .bv1)
+          )
+    )))
+      := by
+      congr 4
+      apply sound
+      apply Wf.eqv.coh
+      apply Wf.pre_beta_pureIn
+        (hΓ := (((((Γr.erase.erase_left.comm.cons (Var?.SSplit.right { ty := A, q := ⊤ })).cons
+                          (Var?.SSplit.right { ty := B, q := ⊤ })).cons
+                      (Var?.SSplit.left { ty := C, q := ⊤ })).s1_23_13
+                  (((Γr.erase.erase.erase_left.comm.cons (Var?.SSplit.left { ty := A, q := ⊤ })).cons
+                        (Var?.SSplit.right { ty := B, q := ⊤ })).cons
+                    (Var?.SSplit.right _))).cons
+              (Var?.SSplit.left { ty := A, q := ⊤ })))
+          .bv2 ⊤ _
+          (b := (.pair (((Ctx?.erase_left _).cons (.left _)).cons (.right _)) .bv1
+            (.pair ((Ctx?.erase_left _).cons (.left _)) .bv0 .bv2)))
+      simp; simp [quant]
+      simp [Wf.let₁, Wf.pair, Wf.pwk, Wf.subst, Wf.bv1, Wf.bv2]; rfl
+    _ = let₁ (hΓ.s12_3_1_23 hΓc).comm a
+    (let₁ ((hΓ.s12_3_23 hΓc).comm.cons (Var?.SSplit.left { ty := A, q := ⊤ })) (wk0 _ b)
+      (let₁
+        ((Γr.erase_right.comm.cons
+        (Var?.SSplit.left { ty := A, q := ⊤ })).cons (Var?.SSplit.left { ty := B, q := ⊤ }))
+        (wk0 _ (wk0 _ c))
+          (
+            .pair (((Ctx?.erase_right _).cons (.right _)).cons (.right _)) .bv2
+              (.pair (((Ctx?.erase_right _).cons (.left _)).cons (.right _)) .bv1 .bv0)
+          )
+        )) := by
+      congr 3
+      apply sound
+      apply Wf.eqv.coh
+      apply Wf.pre_beta_pureIn
+        (hΓ := ((((Γr.erase.erase_left.comm.cons (Var?.SSplit.right { ty := A, q := ⊤ })).cons
+                    (Var?.SSplit.right { ty := B, q := ⊤ })).cons
+                (Var?.SSplit.left { ty := C, q := ⊤ })).s1_23_13_2
+            (((Γr.erase.erase.erase_left.comm.cons (Var?.SSplit.left { ty := A, q := ⊤ })).cons
+                  (Var?.SSplit.right { ty := B, q := ⊤ })).cons
+              (Var?.SSplit.right _))))
+        .bv2 ⊤ _
+        (b :=
+          (
+            .pair ((Ctx?.erase_left _).cons (.left _)) .bv0
+              (.pair ((((Ctx?.erase_left _).cons (.left _)).cons (.right _)).cons (.right _))
+                .bv2
+                .bv1)
+          ))
+      simp; simp [quant]
+      simp [Wf.let₁, Wf.pair, Wf.pwk, Wf.subst]; rfl
+  _ = _ :=  by
+    conv => rhs; rw [bind_pair]; rhs; lhs; rw [wk0_pair, bind_pair]
+    rw [bind_pair_right _ ⊥ ⊤, let_let₁, let_let₁]
+    congr 1
+    induction b, c using quotInd₂
+    apply sound; apply Wf.eqv.of_tm
+    simp [Wf.let₁, Wf.wk0, Wf.pair, Wf.bv0, Wf.wk1, Wf.bv2, Wf.bv1]
+    apply HasCommRel.commutes_bot_left
+
+theorem Eqv.reassoc_reassoc_inv {Γ : Ctx? α} {A B C : Ty α}
+  (a : Eqv R Γ (A.tensor (B.tensor C)))
+  : a.reassoc_inv.reassoc = a
+  := calc
+  _ = a.eta_assoc_inv := by
+    rw [reassoc_inv, let₂_reassoc, let₂_reassoc, reassoc_beta]
+    induction a using quotInd
+    exact Eqv.of_tm rfl
+  _ = _ := by rw [a.eta_assoc_inv_eq_id]
+
+theorem Eqv.reassoc_inv_injective {Γ : Ctx? α} {A B C : Ty α}
+  (a b : Eqv R Γ (A.tensor (B.tensor C)))
+  (h : a.reassoc_inv = b.reassoc_inv) : a = b
+  := by rw [<-a.reassoc_reassoc_inv, <-b.reassoc_reassoc_inv, h]
+
+theorem Eqv.reassoc_inv_reassoc {Γ : Ctx? α} {A B C : Ty α}
+  (a : Eqv R Γ ((A.tensor B).tensor C))
+  : a.reassoc.reassoc_inv = a
+  := by calc
+  _ = a.eta_assoc := by
+    rw [eta_assoc, reassoc, letT₂, let₂_reassoc_inv, let₂_reassoc_inv]
+    congr 2
+    rw [
+      reassoc_inv, let₂_beta, wk0_pair, wk0_bv0, wk0_bv2,
+      let₂_let₁_bv0_anti'
+        (c' :=
+          (.pair (Ctx?.erase_right _).right (.pair (Ctx?.erase_right _).right.right .bv2 .bv1) .bv0)
+        )
+        (hc := by apply Eqv.of_tm; simp [Wf.pair, Wf.wk2, Wf.bv1, Wf.bv0, Wf.bv2, Wf.bv3]),
+      let₂_beta
+    ]
+    conv => rhs; lhs; rw [bind_pair]
+    rw [let_pair_right, let_pair_right]
+    conv => rhs; rhs; rhs; rw [
+      bind_pair_right _ ⊥ ⊤ (ha := inferInstance) (hb := inferInstance)
+        (he := HasCommRel.commutes_bot_left),
+    ]
+    apply Eqv.of_tm
+    simp [Wf.let₁, Wf.bv1, Wf.wk0, Wf.bv0, Wf.bv2, Wf.bv3, Wf.pwk, Wf.pair]
+  _ = _ := by rw [a.eta_assoc_eq_id]
+
+theorem Eqv.reassoc_injective {Γ : Ctx? α} {A B C : Ty α}
+  (a b : Eqv R Γ ((A.tensor B).tensor C))
+  (h : a.reassoc = b.reassoc) : a = b
+  := by rw [<-a.reassoc_inv_reassoc, <-b.reassoc_inv_reassoc, h]
+
+theorem Eqv.reassoc_inv_beta {Γ Γc Γl Γm Γr : Ctx? α} {A B C : Ty α}
+  (hΓ : Γ.SSplit Γl Γc) (hΓc : Γc.SSplit Γm Γr)
+  (a : Eqv R Γl A) (b : Eqv R Γm B) (c : Eqv R Γr C)
+  : (a.pair hΓ (b.pair hΓc c)).reassoc_inv = (a.pair (hΓ.s1_23_12 hΓc) b).pair (hΓ.s1_23_12_3 hΓc) c
+  := by
+  apply reassoc_injective
+  rw [reassoc_reassoc_inv, reassoc_beta]
+  induction a, b, c using quotInd₃
+  exact Eqv.of_tm rfl
+
+theorem DRWS.Obj.assoc_comp_assoc_inv {A B C : R.Obj}
+  : (DRWS.Obj.assoc A B C).comp (DRWS.Obj.assoc_inv A B C) = id ((A.tensor B).tensor C) := by
+  simp [DRWS.Arrow.comp, Eqv.letArrow_assoc_inv, DRWS.Obj.assoc, Eqv.reassoc_inv_reassoc]
+  rfl
+
+theorem DRWS.Obj.assoc_inv_comp_assoc {A B C : R.Obj}
+  : (DRWS.Obj.assoc_inv A B C).comp (DRWS.Obj.assoc A B C) = id (A.tensor (B.tensor C)) := by
+  simp [DRWS.Arrow.comp, Eqv.letArrow_assoc, DRWS.Obj.assoc_inv, Eqv.reassoc_reassoc_inv]
+  rfl
+
+open CategoryTheory
+
+instance DRWS.Obj.instMonoidalCategoryStruct : MonoidalCategoryStruct R.Obj where
+  tensorObj A B := A.tensor B
+  tensorUnit := .unit
+  tensorHom f g := f.tensorHom g
+  whiskerLeft A _ _ f := f.whiskerLeft A
+  whiskerRight f B := f.whiskerRight B
+  associator A B C :=
+    ⟨A.assoc B C, A.assoc_inv B C, DRWS.Obj.assoc_comp_assoc_inv, DRWS.Obj.assoc_inv_comp_assoc⟩
+  leftUnitor A :=
+    ⟨A.leftUnitor, A.leftUnitor_inv,
+      DRWS.Obj.leftUnitor_leftUnitor_inv, DRWS.Obj.leftUnitor_inv_leftUnitor⟩
+  rightUnitor A :=
+    ⟨A.rightUnitor, A.rightUnitor_inv,
+      DRWS.Obj.rightUnitor_rightUnitor_inv, DRWS.Obj.rightUnitor_inv_rightUnitor⟩
