Refinery/Term/Extrinsic/Wf/LetThen.lean
@@ -1,4 +1,4 @@
-import Refinery.Term.Extrinsic.Wf.Rewrite
+import Refinery.Term.Extrinsic.Wf.DerivedRewrite
 
 open HasQuant HasPQuant HasCommRel
 
@@ -29,3 +29,25 @@ def Eqv.letT₂_eta {Γ : Ctx? α} {A B : Ty α}
   (a : Eqv R Γ (A.tensor B))
   : a.letT₂ (.pair (((Γ.erase.both).cons (.left _)).cons (.right _)) .bv1 .bv0)
   = a := a.let₂_eta
+
+variable [R.UWkCongr]
+
+theorem Eqv.letT₂_letT₂ {Γ : Ctx? α} {A B C D E : Ty α}
+  (a : Eqv R Γ (A.tensor B))
+  (b : Eqv R ((Γ.erase.cons ⟨A, ⊤⟩).cons ⟨B, ⊤⟩) (C.tensor D))
+  (c : Eqv R ((Γ.erase.cons ⟨C, ⊤⟩).cons ⟨D, ⊤⟩) E)
+  : (a.letT₂ b).letT₂ c
+  = a.letT₂ (b.letT₂ (((c.castCtx (by (conv => lhs; rw [<-Ctx?.erase_erase]); rfl)).wk2 _).wk2 _))
+  := by
+  rw [letT₂, letT₂, let₂_let₂]
+  induction a, b, c using quotInd₃
+  exact of_tm rfl
+
+theorem Eqv.letT₂_beta  {Γ Γl Γr : Ctx? α} {A B}
+  (hΓ : Γ.SSplit Γl Γr) (a : Eqv R Γl A) (b : Eqv R Γr B)
+  (c : Eqv R ((Γ.erase.cons ⟨A, ⊤⟩).cons ⟨B, ⊤⟩) C)
+  : letT₂ (pair hΓ a b) c = .let₁ hΓ.comm a (.let₁ (Ctx?.erase_left _).left (b.wk0 _)
+    (c.castCtx (by rw [hΓ.erase_eq_right]))) := by
+  rw [letT₂, let₂_beta]
+  induction a, b, c using quotInd₃
+  exact of_tm rfl
